Task 2.2

hws/assn0/assn0.lean
@@ -22,15 +22,35 @@ inductive stack : Type :=
 | cons : card → stack → stack
 
 namespace stack
-  open card
-
   notation h :: t  := cons h t
   notation `[` l:(foldr `, ` (h t, cons h t) nil `]`) := l
 
   inductive unshuffle : stack → stack → stack → Prop :=
   | intro_nil : unshuffle [] [] []
-  | intro_right : ∀ c s₁ s₂ s₃,
+  | intro_right : ∀ {c s₁ s₂ s₃},
                       unshuffle s₁ s₂ s₃ → unshuffle (c :: s₁) s₂ (c :: s₃)
-  | intro_left : ∀ c s₁ s₂ s₃,
+  | intro_left : ∀ {c s₁ s₂ s₃},
                      unshuffle s₁ s₂ s₃ → unshuffle (c :: s₁) (c :: s₂) s₃
+
+  namespace unshuffle
+    notation `🂠🂠🂠` := intro_nil
+    notation `🂡🂠🂡` := intro_right
+    notation `🂡🂡🂠` := intro_left
+  end unshuffle
 end stack
+
+/- Task 2.1 -/
+section
+  open card stack stack.unshuffle function
+
+  example : unshuffle [♡, ♠, ♠, ♢] [♠, ♢] [♡, ♠] :=
+  🂡🂠🂡 $ 🂡🂡🂠 $ 🂡🂠🂡 $ 🂡🂡🂠 $ 🂠🂠🂠
+end
+
+/- Task 2.2 -/
+section
+  open card stack stack.unshuffle function
+
+  example : unshuffle [♡, ♠, ♠, ♢] [♠, ♢] [♡, ♠] :=
+  🂡🂠🂡 $ 🂡🂠🂡 $ 🂡🂡🂠 $ 🂡🂡🂠 $ 🂠🂠🂠
+end
